MECMAR/spec/Semantics.v
@@ -2,45 +2,57 @@ From Coq Require Import PeanoNat ZArith Bool Lia Program.Equality.
 From Warblre Require Import Tactics Focus Result Base Patterns StaticSemantics Notation.
 
 Import Result.Notations.
+Import NoI.Coercions.
 Local Open Scope result_flow.
 
-(** 22.2.2.2 Runtime Semantics: CompilePattern *)
+(** 22.2.2 Pattern Semantics *)
 Module Semantics.
   Import Patterns.
   Import Notation.
 
-  (** 22.2.2.3.1 RepeatMatcher ( m, min, max, greedy, x, c, parenIndex, parenCount ) *)
-  Fixpoint repeatMatcher' (m: Matcher) (min: non_neg_integer) (max: non_neg_integer_or_inf) (greedy: bool) (x: MatchState) (c: MatcherContinuation) (groupsWithin: IdSet.t) (fuel: nat): MatchResult :=
+  (* Some coercions *)
+  (* This one is used implicitly by the specification *)
+  Coercion SomeCR: CaptureRange >-> CaptureRange_or_undefined.
+  (* These are used to wrap things into the error monad we will be using *)
+  Coercion wrap_CaptureRange(cr: CaptureRange) := @Success _ MatchError cr.
+  Coercion state_to_result(x: MatchState) := @Success _ MatchError (Some x).
+
+  (** 22.2.2.3.1 RepeatMatcher ( m, min, max, greedy, x, c, parenIndex, parenCount )
+      The abstract operation RepeatMatcher takes arguments m (a Matcher), min (a non-negative integer), max (a non-
+      negative integer or +∞), greedy (a Boolean), x (a MatchState), c (a MatcherContinuation), parenIndex (a non-negative 
+      integer), and parenCount (a non-negative integer) and returns a MatchResult. It performs the following steps when 
+      called:
+    *)
   (* Coq wants to make sure the function will terminate; we do so by bounding recursion by an arbitrary fuel amount *)
+  Fixpoint repeatMatcher' (m: Matcher) (min: non_neg_integer) (max: non_neg_integer_or_inf) (greedy: bool) (x: MatchState) (c: MatcherContinuation) (groupsWithin: IdSet.t) (fuel: nat): MatchResult :=
   match fuel with
   | 0 => out_of_fuel
   | S fuel' =>
     (* 1. If max = 0, return c(x). *)
-    if max is (Some 0) then c x else
+    if (max =? 0)%NoI then c x else
     (* 2. Let d be a new MatcherContinuation with parameters (y) that captures m, min, max, greedy, x, c, parenIndex, and parenCount and performs the following steps when called: *)
     let d := fun (y: MatchState) =>
       (* a. Assert: y is a MatchState. *)
       (* b. If min = 0 and y's endIndex = x's endIndex, return failure. *)
-      if (Nat.eqb min 0) && ((MatchState.endIndex y) =? (MatchState.endIndex x))%Z 
+      if (min =? 0)%nat && (MatchState.endIndex y =? MatchState.endIndex x)%Z
         then failure else
       (* c. If min = 0, let min2 be 0; otherwise let min2 be min - 1. *)
       let min2 :=
-        if Nat.eqb min 0 then 0
+        if (min =? 0)%nat then 0
         else min - 1
       in
-      (* TODO: improve *)
       (* d. If max = +∞, let max2 be +∞; otherwise let max2 be max - 1. *)
-      let max2 := match max with
-        | None => +∞
-        | Some n => Some (n -1)
-      end in
+      let max2 :=
+        if (max =? +∞)%NoI then +∞
+        else (max - 1)%NoI
+      in
       (* e. Return RepeatMatcher(m, min2, max2, greedy, y, c, parenIndex, parenCount). *)
       repeatMatcher' m min2 max2 greedy y c groupsWithin fuel'
     in
     (* 3. Let cap be a copy of x's captures List. *)
     let cap := MatchState.captures x in
     (* 4. For each integer k in the inclusive interval from parenIndex + 1 to parenIndex + parenCount, set cap[k] to undefined. *)
-    let cap := IdSet.fold DMap.remove groupsWithin cap in
+    set cap[groupsWithin ...] := undefined in
     (* 5. Let Input be x's input. *)
     let input := MatchState.input x in
     (* 6. Let e be x's endIndex. *)
@@ -48,21 +60,23 @@ Module Semantics.
     (* 7. Let xr be the MatchState (Input, e, cap). *)
     let xr := MatchState.make input e cap in
     (* 8. If min ≠ 0, return m(xr, d). *)
-    if negb (Nat.eqb min 0) 
+    if (min !=? 0)%nat
       then m xr d else
     (* 9. If greedy is false, then *)
     if greedy is false then
       (* a. Let z be c(x). *)
       let z := c x in
       (* b. If z is not failure, return z. *)
-      if z is not failure then z else
+      if z is not failure
+        then z else
       (* c. Return m(xr, d).*)
       m xr d
     else
     (* 10. Let z be m(xr, d). *)
     let z := m xr d in
     (* 11. If z is not failure, return z. *)
-    if z is not failure then z else
+    if z is not failure
+      then z else
     (* 12. Return c(x). *)
     c x
   end.
@@ -74,19 +88,18 @@ Module Semantics.
   Fixpoint compileSubPattern (self: Regex) (rer: RegExp) (direction: direction): Matcher := match self with
   | Char A invert =>  (** 22.2.2.7.1 CharacterSetMatcher ( rer, A, invert, direction ) *)
                       (* 1. Return a new Matcher with parameters (x, c) that captures rer, A, invert, and direction and performs the following steps when called: *)
-                      (* a. Assert: x is a MatchState. *)
-                      (* b. Assert: c is a MatcherContinuation. *)
                       fun (x: MatchState) (c: MatcherContinuation) =>
+                        (* a. Assert: x is a MatchState. *)
+                        (* b. Assert: c is a MatcherContinuation. *)
                         (* c. Let Input be x's input. *)
                         let input := MatchState.input x in
                         (* d. Let e be x's endIndex. *)
                         let e := MatchState.endIndex x in
-                        let f :=
-                          (* e. If direction is forward, let f be e + 1. *)
-                          (if Direction.eqb direction forward
-                          then e + 1
-                          (* f. Else, let f be e - 1. *)
-                          else e - 1)%Z
+                        (* e. If direction is forward, let f be e + 1. *)
+                        (* f. Else, let f be e - 1. *)
+                        let f := if direction is forward
+                          then (e + 1)%Z
+                          else (e - 1)%Z
                         in
                         (* g. Let InputLength be the number of elements in Input. *)
                         let inputLength := Z.of_nat (length input) in
@@ -94,44 +107,44 @@ Module Semantics.
                         if (f <? 0)%Z || (f >? inputLength)%Z then
                           failure
                         else
-                          (* i. Let index be min(e, f). *)
-                          let index := Z.min e f in
-                          (* j. Let ch be the character Input[index]. *)
-                          let! chr =<< input[ index ] in
-                          (* k. Let cc be Canonicalize(rer, ch). *)
-                          let cc := chr in
-                          (* l. If there exists a member a of A such that Canonicalize(rer, a) is cc, let found be true. Otherwise, let found be false. *)
-                          let found := A cc in
-                          (* m. If invert is false and found is false, return failure. *)
-                          if Bool.eqb invert false && Bool.eqb found false then
-                            failure
-                          (* n. If invert is true and found is true, return failure. *)
-                          else if Bool.eqb invert true && Bool.eqb found true then
-                            failure
-                          else
-                            (* o. Let cap be x's captures List. *)
-                            let cap := MatchState.captures x in
-                            (* p. Let y be the MatchState (Input, f, cap). *)
-                            let y := match_state input f cap in
-                            (* q. Return c(y). *)
-                            c y
-  | Disjunction r1 r2 =>
+                        (* i. Let index be min(e, f). *)
+                        let index := Z.min e f in
+                        (* j. Let ch be the character Input[index]. *)
+                        let! chr =<< input[ index ] in
+                        (* k. Let cc be Canonicalize(rer, ch). *)
+                        let cc := chr in
+                        (* l. If there exists a member a of A such that Canonicalize(rer, a) is cc, let found be true. Otherwise, let found be false. *)
+                        let found := A cc in
+                        (* m. If invert is false and found is false, return failure. *)
+                        if Bool.eqb invert false && Bool.eqb found false then
+                          failure
+                        (* n. If invert is true and found is true, return failure. *)
+                        else if Bool.eqb invert true && Bool.eqb found true then
+                          failure
+                        else
+                        (* o. Let cap be x's captures List. *)
+                        let cap := MatchState.captures x in
+                        (* p. Let y be the MatchState (Input, f, cap). *)
+                        let y := match_state input f cap in
+                        (* q. Return c(y). *)
+                        c y
+  | Disjunction r1 r2 => (** 22.2.2.3 Runtime Semantics: CompileSubpattern *)
                       (* 1. Let m1 be CompileSubpattern of Alternative with arguments rer and direction. *)
                       let m1 := compileSubPattern r1 rer direction in
                       (* 2. Let m2 be CompileSubpattern of Disjunction with arguments rer and direction. *)
                       let m2 := compileSubPattern r2 rer direction in
                       (* 3. Return a new Matcher with parameters (x, c) that captures m1 and m2 and performs the following steps when called: *)
-                      (* a. Assert: x is a MatchState. *)
-                      (* b. Assert: x is a MatchState. *)
                       fun (x: MatchState) (c: MatcherContinuation) =>
+                        (* a. Assert: x is a MatchState. *)
+                        (* b. Assert: x is a MatchState. *)
                         (* c. Let r be m1(x, c). *)
                         let r := m1 x c in
                         (* d. If r is not failure, return r. *)
                         if r is not failure then
                           r
                         else
-                          (* e. Return m2(x, c). *)
-                          m2 x c
+                        (* e. Return m2(x, c). *)
+                        m2 x c
   | Kleene r      =>  let m := compileSubPattern r rer direction in
                       let groups := capturingGroupsWithin r in
                       fun (x: MatchState) (c: MatcherContinuation) =>
@@ -144,12 +157,12 @@ Module Semantics.
                       (* 3. If direction is forward, then *)
                       if direction is forward then
                         (* a. Return a new Matcher with parameters (x, c) that captures m1 and m2 and performs the following steps when called: *)
-                        (* i. Assert: x is a MatchState. *)
-                        (* ii. Assert: c is a MatcherContinuation. *)
                         fun (s: MatchState) (c: MatcherContinuation) =>
+                          (* i. Assert: x is a MatchState. *)
+                          (* ii. Assert: c is a MatcherContinuation. *)
                           (* iii. Let d be a new MatcherContinuation with parameters (y) that captures c and m2 and performs the following steps when called: *)
-                          (* 1. Assert: y is a MatchState. *)
                           let d := fun (s: MatchState) => 
+                            (* 1. Assert: y is a MatchState. *)
                             (* 2. Return m2(y, c). *)
                             m2 s c
                           in
@@ -159,13 +172,13 @@ Module Semantics.
                       else
                         (* a. Assert: direction is backward. *)
                         (* b. Return a new Matcher with parameters (x, c) that captures m1 and m2 and performs the following steps when called: *)
-                        (* i. Assert: x is a MatchState. *)
-                        (* ii. Assert: x is a MatchState. *)
                         fun (s: MatchState) (c: MatcherContinuation) =>
+                          (* i. Assert: x is a MatchState. *)
+                          (* ii. Assert: x is a MatchState. *)
                           (* iii. Let d be a new MatcherContinuation with parameters (y) that captures c and m1 and performs the following steps when called: *)
-                          (* 1. Assert: y is a MatchState. *)
                           let d := fun (s: MatchState) =>
-                            (* Return m1(y, c). *)
+                            (* 1. Assert: y is a MatchState. *)
+                            (* 2. Return m1(y, c). *)
                             m1 s c 
                           in
                           (* iv. Return m2(x, d). *)
@@ -176,12 +189,12 @@ Module Semantics.
                       (* 2. Let parenIndex be CountLeftCapturingParensBefore(Atom). *)
                       let parenIndex := id in
                       (* 3. Return a new Matcher with parameters (x, c) that captures direction, m, and parenIndex and performs the following steps when called: *)
-                      (* a. Assert: x is a MatchState. *)
-                      (* b. Assert: c is a MatcherContinuation. *)
-                      fun (x: MatchState) (c: MatcherContinuation) => 
+                      fun (x: MatchState) (c: MatcherContinuation) =>
+                        (* a. Assert: x is a MatchState. *)
+                        (* b. Assert: c is a MatcherContinuation. *)
                         (* c. Let d be a new MatcherContinuation with parameters (y) that captures x, c, direction, and parenIndex and performs the following steps when called: *)
-                        (* i. Assert: y is a MatchState. *)
-                        let d := fun (y: MatchState) => 
+                        let d := fun (y: MatchState) =>
+                          (* i. Assert: y is a MatchState. *)
                           (* ii. Let cap be a copy of y's captures List. *)
                           let cap := MatchState.captures y in
                           (* iii. Let Input be x's input. *)
@@ -196,18 +209,17 @@ Module Semantics.
                               (* 1. Assert: xe ≤ ye. *)
                               assert! (xe <=? ye)%Z ;
                               (* 2. Let r be the CaptureRange (xe, ye). *)
-                              Success (CaptureRange.make xe ye)
+                              CaptureRange.make xe ye
                             (* vii. Else, *)
                             else
                               (* 1. Assert: direction is backward. *)
-                              assert! direction is backward ;
                               (* 2. Assert: ye ≤ xe. *)
                               assert! (ye <=? xe)%Z ;
                               (* 3. Let r be the CaptureRange (ye, xe). *)
-                              Success (CaptureRange.make ye xe)
+                              CaptureRange.make ye xe
                           in
                           (* viii. Set cap[parenIndex + 1] to r. *)
-                          let cap := DMap.add id r cap in
+                          set cap[id] := r in
                           (* ix. Let z be the MatchState (Input, ye, cap). *)
                           let z := match_state input ye cap in
                           (* x. Return c(z). *)
@@ -219,14 +231,14 @@ Module Semantics.
                       (* 1. Let m be CompileSubpattern of Disjunction with arguments rer and backward. *)
                       let m := compileSubPattern r rer backward in
                       (* 2. Return a new Matcher with parameters (x, c) that captures m and performs the following steps when called: *)
-                      (* a. Assert: x is a MatchState. *)
-                      (* b. Assert: c is a MatcherContinuation. *)
                       fun (x: MatchState) (c: MatcherContinuation) =>
+                        (* a. Assert: x is a MatchState. *)
+                        (* b. Assert: c is a MatcherContinuation. *)
                         (* c. Let d be a new MatcherContinuation with parameters (y) that captures nothing and performs the following steps when called: *)
-                        (* i. Assert: y is a MatchState. *)
                         let d := fun (y: MatchState) =>
+                          (* i. Assert: y is a MatchState. *)
                           (* ii. Return y. *)
-                          Success (Some y)
+                          y
                         in
                         (* d. Let r be m(x, d). *)
                         let r := m x d in
@@ -234,43 +246,42 @@ Module Semantics.
                         if r is failure then
                           failure
                         else
-                          (* f. Let y be r's MatchState. *)
-                          destruct! Success (Some y) <- r in
-                          (* g. Let cap be y's captures List. *)
-                          let cap := MatchState.captures y in
-                          (* h. Let cap be y's captures List. *)
-                          let input := MatchState.input x in
-                          (* i. Let cap be y's captures List. *)
-                          let xe := MatchState.endIndex x in
-                          (* j. Let z be the MatchState (Input, xe, cap). *)
-                          let z := match_state input xe cap in
-                          (* k. Let z be the MatchState (Input, xe, cap). *)
-                          c z
+                        (* f. Let y be r's MatchState. *)
+                        destruct! Success (Some y) <- r in
+                        (* g. Let cap be y's captures List. *)
+                        let cap := MatchState.captures y in
+                        (* h. Let cap be y's captures List. *)
+                        let input := MatchState.input x in
+                        (* i. Let cap be y's captures List. *)
+                        let xe := MatchState.endIndex x in
+                        (* j. Let z be the MatchState (Input, xe, cap). *)
+                        let z := match_state input xe cap in
+                        (* k. Let z be the MatchState (Input, xe, cap). *)
+                        c z
   end.
 
-  (** 22.2.2.2 Runtime Semantics: CompilePattern *)
-  (*  The syntax-directed operation CompilePattern takes argument rer (a RegExp Record) and returns an
+  (** 22.2.2.2 Runtime Semantics: CompilePattern
+      The syntax-directed operation CompilePattern takes argument rer (a RegExp Record) and returns an
       Abstract Closure that takes a List of characters and a non-negative integer and returns a MatchResult. It is
       defined piecewise over the following productions: *)
   Definition compilePattern (r: Regex) (rer: RegExp): list Character -> non_neg_integer -> MatchResult :=
     (* 1. Let m be CompileSubpattern of Disjunction with arguments rer and forward. *)
     let m := compileSubPattern r rer forward in
     (* 2. Return a new Abstract Closure with parameters (Input, index) that captures rer and m and performs the following steps when called: *)
-    (* a. Assert: Input is a List of characters. *)
     fun (input: list Character) (index: non_neg_integer) =>
-      (* Assert: 0 ≤ index ≤ the number of elements in Input. *)
-      assert! PeanoNat.Nat.leb 0 index && PeanoNat.Nat.leb index (length input) ;
+      (* a. Assert: Input is a List of characters. *)
+      (* b. Assert: 0 ≤ index ≤ the number of elements in Input. *)
+      assert! (0 <=? index)%nat && (index <=? (length input))%nat ;
       (* c. Let c be a new MatcherContinuation with parameters (y) that captures nothing and performs the following steps when called: *)
-      (* i. Assert: y is a MatchState. *)
       let c := fun (y: MatchState) =>
-        (* Return y. *)
-        Success (Some y) 
+        (* i. Assert: y is a MatchState. *)
+        (* ii. Return y. *)
+        y
       in
       (* d. Let cap be a List of rer.[[CapturingGroupsCount]] undefined values, indexed 1 through rer.[[CapturingGroupsCount]]. *)
-      let cap := DMap.empty CaptureRange.type in
+      let cap := DMap.empty CaptureRange_or_undefined in
       (* e. Let x be the MatchState (Input, index, cap). *)
       let x := match_state input (Z.of_nat index) cap in
       (* f. Return m(x, c). *)
-      m x c
-    .
+      m x c.
 End Semantics.
